shell.nix
@@ -1,2 +1,2 @@
-args@{ version ? "coq-jlib_8_15" }:
+args@{ version ? "coq-jlib_8_10" }:
 (import ./default.nix args).${version}
